src/impl/TLS13.Handshake.ByteDriver.External.fsti
@@ -10,30 +10,19 @@ module IO = TLS13.IO
 module SZ = FStar.SizeT
 module U8 = FStar.UInt8
 
-type progress =
-  | ExpectEncryptedExtensions
-  | ExpectCertificate
-  | ExpectCertificateVerify
-  | ExpectFinished
-  | Complete
-
 val context : Type0
-val is_context: context -> progress -> slprop
-
-fn reset_encrypted_handshake (ctx: context)
-  requires is_context ctx 'p
-  ensures is_context ctx ExpectEncryptedExtensions
+val is_context: context -> slprop
 
 fn read_raw (ctx: context) (ch: IO.channel) (buf: array U8.t)
   (total_len: SZ.t) (offset: SZ.t) (remaining: SZ.t)
-  requires is_context ctx 'p ** IO.is_channel ch
+  requires is_context ctx ** IO.is_channel ch
            ** pts_to buf 'old
            ** pure (B.length 'old == SZ.v total_len /\
                     SZ.v remaining > 0 /\
                     SZ.v offset + SZ.v remaining <= SZ.v total_len)
   returns n: SZ.t
   ensures exists* bytes.
-          is_context ctx 'p ** IO.is_channel ch
+          is_context ctx ** IO.is_channel ch
           ** pts_to buf bytes
           ** pure (B.length bytes == SZ.v total_len /\
                    SZ.v n <= SZ.v remaining)
